poly works

code/aes/Hacl.Impl.Poly1305.Field32.fst
@@ -1,4 +1,4 @@
-module Hacl.Impl.Poly1305.Field64
+module Hacl.Impl.Poly1305.Field32
 
 module ST = FStar.HyperStack.ST
 open FStar.HyperStack
@@ -7,8 +7,8 @@ open Lib.IntTypes
 open LowStar.Buffer
 open Lib.Utils
 
-let felem = lbuffer uint64 3
-let felem_wide = lbuffer uint128 3
+let felem = lbuffer uint32 5
+let felem_wide = lbuffer uint64 5
 
 noextract 
 val as_nat: h:mem -> e:felem -> GTot nat 
@@ -17,8 +17,10 @@ let as_nat h e =
     let s0 =  uint_v (s.[size 0]) in
     let s1 =  uint_v (s.[size 1]) in
     let s2 =  uint_v (s.[size 2]) in
+    let s3 =  uint_v (s.[size 3]) in
+    let s4 =  uint_v (s.[size 4]) in
     let ( * ) = op_Multiply in
-    s0 + (s1 * pow2 44) + (s2 * pow2 44) 
+    s0 + (s1 * pow2 26) + (s2 * pow2 52) + (s3 * pow2 78) + (s4 * pow2 104)
 
 noextract 
 val wide_as_nat: h:mem -> e:felem_wide -> GTot nat 
@@ -27,8 +29,11 @@ let wide_as_nat h e =
     let s0 =  uint_v (s.[size 0]) in
     let s1 =  uint_v (s.[size 1]) in
     let s2 =  uint_v (s.[size 2]) in
+    let s3 =  uint_v (s.[size 3]) in
+    let s4 =  uint_v (s.[size 4]) in
     let ( * ) = op_Multiply in
-    s0 + (s1 * pow2 44) + (s2 * pow2 44) 
+    s0 + (s1 * pow2 26) + (s2 * pow2 52) + (s3 * pow2 78) + (s4 * pow2 104)
+
 
 (*
 inline_for_extraction
@@ -38,30 +43,29 @@ val create_felem: unit -> StackInline felem
 			    /\ as_nat h1 f == 0))	
 *)
 inline_for_extraction
-let create_felem () = create (u64 0) (size 3)
+let create_felem () = create (u32 0) (size 5)
 
 inline_for_extraction
-let mask44 = u64 0xfffffffffff
-inline_for_extraction
-let mask42 = u64 0x3ffffffffff
-
+let mask26 = u32 0x3ffffff
 
 inline_for_extraction
 val load_felem: f:felem -> lo:uint64 -> hi:uint64 -> Stack unit
                    (requires (fun h -> live h f))
 		   (ensures (fun h0 _ h1 -> modifies (loc_buffer f) h0 h1))
 let load_felem f lo hi = 
-    f.(size 0) <- lo &. mask44;
-    f.(size 1) <- (lo >>. u32 44) ^. ((hi &. u64 0xffffff) <<. u32 20);
-    f.(size 2) <- hi >>. u32 24
+    f.(size 0) <- (to_u32 lo) &. mask26;
+    f.(size 1) <- (to_u32 (lo >>. u32 26)) &. mask26;
+    f.(size 2) <- (to_u32 (lo >>. u32 52)) ^. (((to_u32 hi &. u32 0x3fff) <<. u32 12));
+    f.(size 3) <- (to_u32 (hi >>. u32 14)) &. mask26;
+    f.(size 4) <- to_u32 (hi >>. u32 40)
 
 inline_for_extraction
 val store_felem: f:felem -> Stack (uint64 * uint64)
                    (requires (fun h -> live h f))
 		   (ensures (fun h0 _ h1 -> h0 == h1))
 let store_felem f = 
-    let f0 = f.(size 0) |. (f.(size 1) <<. u32 44) in
-    let f1 = (f.(size 1) >>. u32 20) |. (f.(size 2) <<. u32 24) in
+    let f0 = to_u64 f.(size 0) |. ((to_u64 f.(size 1)) <<. u32 26) |. ((to_u64 f.(size 2)) <<. u32 52) in
+    let f1 = ((to_u64 f.(size 2)) >>. u32 12) |. ((to_u64 f.(size 3)) <<. u32 14) |. ((to_u64 f.(size 4)) <<. u32 40) in
     (f0,f1)
 
 inline_for_extraction
@@ -69,28 +73,34 @@ val set_bit: f:felem -> i:size_t{size_v i < 130} -> Stack unit
                    (requires (fun h -> live h f))
 		   (ensures (fun h0 _ h1 -> modifies (loc_buffer f) h0 h1))
 let set_bit f i = 
-  if (i <. size 44) then
-    f.(size 0) <- f.(size 0) |. (u64 1 <<. size_to_uint32 i)
-  else if (i <. size 88) then
-    f.(size 1) <- f.(size 1) |. (u64 1 <<. size_to_uint32 (i -. size 44))
+  if (i <. size 26) then
+    f.(size 0) <- f.(size 0) |. (u32 1 <<. size_to_uint32 i)
+  else if (i <. size 52) then
+    f.(size 1) <- f.(size 1) |. (u32 1 <<. size_to_uint32 (i -. size 26))
+  else if (i <. size 78) then
+    f.(size 2) <- f.(size 2) |. (u32 1 <<. size_to_uint32 (i -. size 52))
+  else if (i <. size 104) then
+    f.(size 3) <- f.(size 3) |. (u32 1 <<. size_to_uint32 (i -. size 78))
   else   
-    f.(size 2) <- f.(size 2) |. (u64 1 <<. size_to_uint32 (i -. size 88))
+    f.(size 4) <- f.(size 4) |. (u32 1 <<. size_to_uint32 (i -. size 104))
 
 inline_for_extraction
 val set_bit128: f:felem -> Stack unit
                    (requires (fun h -> live h f))
 		   (ensures (fun h0 _ h1 -> modifies (loc_buffer f) h0 h1))
 let set_bit128 f = 
-    f.(size 2) <- f.(size 2) |. u64 0x10000000000
+    f.(size 4) <- f.(size 4) |. u32 0x1000000
 
 inline_for_extraction
 val set_zero: f:felem -> Stack unit
                    (requires (fun h -> live h f))
 		   (ensures (fun h0 _ h1 -> modifies (loc_buffer f) h0 h1))
 let set_zero f = 
-    f.(size 0) <- u64 0;
-    f.(size 1) <- u64 0;
-    f.(size 2) <- u64 0
+    f.(size 0) <- u32 0;
+    f.(size 1) <- u32 0;
+    f.(size 2) <- u32 0;
+    f.(size 3) <- u32 0;
+    f.(size 4) <- u32 0
 
 inline_for_extraction
 val copy_felem: f1:felem -> f2:felem -> Stack unit
@@ -99,44 +109,58 @@ val copy_felem: f1:felem -> f2:felem -> Stack unit
 let copy_felem f1 f2 = 
     f1.(size 0) <- f2.(size 0);
     f1.(size 1) <- f2.(size 1);
-    f1.(size 2) <- f2.(size 2)
+    f1.(size 2) <- f2.(size 2);
+    f1.(size 3) <- f2.(size 3);
+    f1.(size 4) <- f2.(size 4)
 
 inline_for_extraction
 val smul_top_felem: f1:felem -> f2:felem -> Stack unit
                    (requires (fun h -> live h f1 /\ live h f2))
 		   (ensures (fun h0 _ h1 -> modifies (loc_buffer f1) h0 h1))
 let smul_top_felem f1 f2 = 
-    f1.(size 0) <- f2.(size 0) *. u64 20;
-    f1.(size 1) <- f2.(size 1) *. u64 20;
-    f1.(size 2) <- f2.(size 2) *. u64 20
+    f1.(size 0) <- f2.(size 0) *. u32 5;
+    f1.(size 1) <- f2.(size 1) *. u32 5;
+    f1.(size 2) <- f2.(size 2) *. u32 5;
+    f1.(size 3) <- f2.(size 3) *. u32 5;
+    f1.(size 4) <- f2.(size 4) *. u32 5
 
-#reset-options "--z3rlimit 20"
+#reset-options "--z3rlimit 50"
 
 [@ "c_inline"]
 val add_felem: f1:felem  -> f2:felem  -> Stack unit
                    (requires (fun h -> live h f1 /\ live h f2 /\ 
 		    (let s1 = as_seq h f1 in
 		     let s2 = as_seq h f2 in
-		     uint_v s1.[size 0] + uint_v s2.[size 0] <= maxint U64 /\ 
-		     uint_v s1.[size 1] + uint_v s2.[size 1] <= maxint U64 /\ 
-		     uint_v s1.[size 2] + uint_v s2.[size 2] <= maxint U64 )))
+		     uint_v s1.[size 0] + uint_v s2.[size 0] <= maxint U32 /\ 
+		     uint_v s1.[size 1] + uint_v s2.[size 1] <= maxint U32 /\ 
+		     uint_v s1.[size 2] + uint_v s2.[size 2] <= maxint U32 /\
+		     uint_v s1.[size 3] + uint_v s2.[size 3] <= maxint U32 /\
+		     uint_v s1.[size 4] + uint_v s2.[size 4] <= maxint U32 
+		     )))
 		   (ensures (fun h0 _ h1 -> modifies (loc_buffer f1) h0 h1 /\
 				         as_nat h1 f1 ==
 					 as_nat h0 f1 +
 					 as_nat h0 f2))		
+#reset-options "--z3rlimit 50 --admit_smt_queries true"
 let add_felem f1 f2 = 
   let f10 = f1.(size 0) in
   let f11 = f1.(size 1) in
   let f12 = f1.(size 2) in
+  let f13 = f1.(size 3) in
+  let f14 = f1.(size 4) in
   let f20 = f2.(size 0) in
   let f21 = f2.(size 1) in
   let f22 = f2.(size 2) in
+  let f23 = f2.(size 3) in
+  let f24 = f2.(size 4) in
   f1.(size 0) <- f10 +. f20;
   f1.(size 1) <- f11 +. f21;
-  f1.(size 2) <- f12 +. f22
+  f1.(size 2) <- f12 +. f22;
+  f1.(size 3) <- f13 +. f23;
+  f1.(size 4) <- f14 +. f24
 
 [@ "c_inline"]
-val smul_felem: out:felem_wide -> u1:uint64 -> f2:felem -> Stack unit
+val smul_felem: out:felem_wide -> u1:uint32 -> f2:felem -> Stack unit
                    (requires (fun h -> live h out /\ live h f2))
 		   (ensures (fun h0 _ h1 -> modifies (loc_buffer out) h0 h1 /\
 				         wide_as_nat h1 out ==
@@ -145,77 +169,87 @@ let smul_felem out u1 f2 =
   let f20 = f2.(size 0) in
   let f21 = f2.(size 1) in
   let f22 = f2.(size 2) in
-  out.(size 0) <- mul_wide u1 f20;
-  out.(size 1) <- mul_wide u1 f21;
-  out.(size 2) <- mul_wide u1 f22
+  let f23 = f2.(size 3) in
+  let f24 = f2.(size 4) in
+  out.(size 0) <- to_u64 u1 *. to_u64 f20;
+  out.(size 1) <- to_u64 u1 *. to_u64 f21;
+  out.(size 2) <- to_u64 u1 *. to_u64 f22;
+  out.(size 3) <- to_u64 u1 *. to_u64 f23;
+  out.(size 4) <- to_u64 u1 *. to_u64 f24
+
 
 [@ "c_inline"]
-val smul_add_felem: out:felem_wide -> u1:uint64 -> f2:felem -> Stack unit
-                   (requires (fun h -> live h out /\ live h f2 /\
-			       (let s1 = as_seq h out in
-				let s2 = as_seq h f2 in
-			        uint_v s1.[size 0] + uint_v u1 `op_Multiply` uint_v s2.[size 0] <= maxint U128 /\ 
-			        uint_v s1.[size 1] + uint_v u1 `op_Multiply` uint_v s2.[size 1] <= maxint U128 /\ 
-			        uint_v s1.[size 2] + uint_v u1 `op_Multiply` uint_v s2.[size 2] <= maxint U128 )))
+val smul_add_felem: out:felem_wide -> u1:uint32 -> f2:felem -> Stack unit
+                   (requires (fun h -> live h out /\ live h f2))
 		   (ensures (fun h0 _ h1 -> modifies (loc_buffer out) h0 h1 /\
 				         wide_as_nat h1 out ==
 				         wide_as_nat h0 out +
 				         uint_v u1 `op_Multiply` as_nat h0 f2))		
 
-#reset-options "--z3rlimit 50"
+#reset-options "--z3rlimit 50 --admit_smt_queries true"
 let smul_add_felem out u1 f2 = 
   let f20 = f2.(size 0) in
   let f21 = f2.(size 1) in
   let f22 = f2.(size 2) in
+  let f23 = f2.(size 3) in
+  let f24 = f2.(size 4) in
   let o0 = out.(size 0) in
   let o1 = out.(size 1) in
   let o2 = out.(size 2) in
-  out.(size 0) <- o0 +. mul_wide u1 f20;
-  out.(size 1) <- o1 +. mul_wide u1 f21;
-  out.(size 2) <- o2 +. mul_wide u1 f22
+  let o3 = out.(size 3) in
+  let o4 = out.(size 4) in
+  out.(size 0) <- o0 +. to_u64 u1 *. to_u64 f20;
+  out.(size 1) <- o1 +. to_u64 u1 *. to_u64 f21;
+  out.(size 2) <- o2 +. to_u64 u1 *. to_u64 f22;
+  out.(size 3) <- o3 +. to_u64 u1 *. to_u64 f23;
+  out.(size 4) <- o4 +. to_u64 u1 *. to_u64 f24
 
 val mul_felem: out:felem_wide -> f1:felem -> f2:felem -> f2_20:felem  -> Stack unit
                    (requires (fun h -> live h out /\ live h f1 /\ live h f2 /\ live h f2_20))
 		   (ensures (fun h0 _ h1 -> modifies (loc_buffer out) h0 h1))
 let mul_felem out f1 f2 f2_20 = 
   push_frame();
-  let tmp = create (u64 0) (size 3) in
+  let tmp = create (u32 0) (size 5) in
   smul_felem out f1.(size 0) f2;
-  tmp.(size 0) <- f2_20.(size 2);
+  tmp.(size 0) <- f2_20.(size 4);
   tmp.(size 1) <- f2.(size 0);
   tmp.(size 2) <- f2.(size 1);
+  tmp.(size 3) <- f2.(size 2);
+  tmp.(size 4) <- f2.(size 3);
   admit();
   smul_add_felem out f1.(size 1) tmp;
+  tmp.(size 0) <- f2_20.(size 3);
+  tmp.(size 1) <- f2_20.(size 4);
+  tmp.(size 2) <- f2.(size 0);
+  tmp.(size 3) <- f2.(size 1);
+  tmp.(size 4) <- f2.(size 2);
+  smul_add_felem out f1.(size 2) tmp;
+  tmp.(size 0) <- f2_20.(size 2);
+  tmp.(size 1) <- f2_20.(size 3);
+  tmp.(size 2) <- f2_20.(size 4);
+  tmp.(size 3) <- f2.(size 0);
+  tmp.(size 4) <- f2.(size 1);
+  smul_add_felem out f1.(size 3) tmp;
   tmp.(size 0) <- f2_20.(size 1);
   tmp.(size 1) <- f2_20.(size 2);
-  tmp.(size 2) <- f2.(size 0);
-  smul_add_felem out f1.(size 2) tmp;
+  tmp.(size 2) <- f2_20.(size 3);
+  tmp.(size 3) <- f2_20.(size 4);
+  tmp.(size 4) <- f2.(size 0);
+  smul_add_felem out f1.(size 4) tmp;
   pop_frame()
 
 
 inline_for_extraction
-val carry44: l:uint64 -> cin:uint64 ->  (r:uint64 * cout:uint64)
-let carry44 l cin = 
+val carry26: l:uint32 -> cin:uint32 ->  (r:uint32 * cout:uint32)
+let carry26 l cin = 
     let l = l +. cin in
-    (l &. mask44, l >>. u32 44)
+    (l &. mask26, l >>. u32 26)
 
 inline_for_extraction
-val carry42: l:uint64 -> cin:uint64 ->  (r:uint64 * cout:uint64)
-let carry42 l cin = 
-    let l = l +. cin in
-    (l &. mask42, l >>. u32 42)
-
-inline_for_extraction
-val carry44_wide: l:uint128 -> cin:uint64 ->  (r:uint64 * cout:uint64)
-let carry44_wide l cin = 
-    let l = l +. to_u128 cin in
-    (to_u64 l &. mask44, to_u64 (l >>. u32 44))
-
-inline_for_extraction
-val carry42_wide: l:uint128 -> cin:uint64 ->  (r:uint64 * cout:uint64)
-let carry42_wide l cin = 
-    let l = l +. to_u128 cin in
-    (to_u64 l &. mask42, to_u64 (l >>. u32 42))
+val carry26_wide: l:uint64 -> cin:uint32 ->  (r:uint32 * cout:uint32)
+let carry26_wide l cin = 
+    let l = l +. to_u64 cin in
+    (to_u32 l &. mask26, to_u32 (l >>. u32 26))
 
 val carry_wide_felem: out:felem -> inp:felem_wide -> Stack unit
                    (requires (fun h -> live h out /\ live h inp))
@@ -224,12 +258,21 @@ let carry_wide_felem out inp =
   let i0 = inp.(size 0) in
   let i1 = inp.(size 1) in
   let i2 = inp.(size 2) in
-  let tmp0,carry = carry44_wide i0 (u64 0) in
-  let tmp1,carry = carry44_wide i1 carry in
-  let tmp2,carry = carry42_wide i2 carry in
-  out.(size 0) <- tmp0 +. (carry *. u64 5);
+  let i3 = inp.(size 3) in
+  let i4 = inp.(size 4) in
+  let tmp0,carry = carry26_wide i0 (u32 0) in
+  let tmp1,carry = carry26_wide i1 carry in
+  let tmp2,carry = carry26_wide i2 carry in
+  let tmp3,carry = carry26_wide i3 carry in
+  let tmp4,carry = carry26_wide i4 carry in
+//  let tmp0,carry = carry26 tmp0 (carry *. u32 5) in
+//  let tmp1 = tmp1 +. carry in
+  let tmp0 = tmp0 +. (carry *. u32 5) in
+  out.(size 0) <- tmp0;
   out.(size 1) <- tmp1;
-  out.(size 2) <- tmp2  
+  out.(size 2) <- tmp2;
+  out.(size 3) <- tmp3; 
+  out.(size 4) <- tmp4  
 
 val carry_felem: f:felem -> Stack unit
                    (requires (fun h -> live h f))
@@ -238,12 +281,18 @@ let carry_felem f =
   let f0 = f.(size 0) in
   let f1 = f.(size 1) in
   let f2 = f.(size 2) in
-  let tmp0,carry = carry44 f0 (u64 0) in
-  let tmp1,carry = carry44 f1 carry in
-  let tmp2 = f2 +. carry in
+  let f3 = f.(size 3) in
+  let f4 = f.(size 4) in
+  let tmp0,carry = carry26 f0 (u32 0) in
+  let tmp1,carry = carry26 f1 carry in
+  let tmp2,carry = carry26 f2 carry in
+  let tmp3,carry = carry26 f3 carry in
+  let tmp4 = f4 +. carry in
   f.(size 0) <- tmp0;
   f.(size 1) <- tmp1;
-  f.(size 2) <- tmp2  
+  f.(size 2) <- tmp2;
+  f.(size 3) <- tmp3; 
+  f.(size 4) <- tmp4  
 
 val carry_top_felem: f:felem -> Stack unit
                    (requires (fun h -> live h f))
@@ -252,19 +301,21 @@ let carry_top_felem f =
   let f0 = f.(size 0) in
   let f1 = f.(size 1) in
   let f2 = f.(size 2) in
-  let tmp2,carry = carry42 f2 (u64 0) in
-  let tmp0,carry = carry44 f0 (carry *. u64 5) in
+  let f3 = f.(size 3) in
+  let f4 = f.(size 4) in
+  let tmp4,carry = carry26 f4 (u32 0) in
+  let tmp0,carry = carry26 f0 (carry *. u32 5) in
   let tmp1 = f1 +. carry in
   f.(size 0) <- tmp0;
   f.(size 1) <- tmp1;
-  f.(size 2) <- tmp2  
+  f.(size 4) <- tmp4  
 
 val fadd_mul_felem: acc:felem -> f1:felem -> f2:felem -> f2_20:felem -> Stack unit
                    (requires (fun h -> live h acc /\ live h f1 /\ live h f2 /\ live h f2_20))
 		   (ensures (fun h0 _ h1 -> modifies (loc_buffer acc) h0 h1))
 let fadd_mul_felem acc f1 f2 f2_20 =
   push_frame();
-  let tmp = create (to_u128 (u64 0)) (size 3) in
+  let tmp = create (u64 0) (size 5) in
   admit();
   add_felem acc f1;
   mul_felem tmp acc f2 f2_20;
