code/aes/Hacl.Impl.Poly1305.Fields.fst
@@ -6,11 +6,12 @@ open FStar.HyperStack.All
 open Lib.IntTypes
 open LowStar.Buffer
 open Lib.Utils
+module F32 = Hacl.Impl.Poly1305.Field32
 module F64 = Hacl.Impl.Poly1305.Field64
 
 type field_spec = 
-  | M32
-  | M64
+  | M32 
+  | M64 
 
 
 unfold
@@ -37,15 +38,21 @@ let nlimb (s:field_spec) : size_nat =
   | M32 -> 5
   | M64 -> 3
 
+unfold
+let blocklen (s:field_spec) : size_nat =
+  match s with
+  | M32 -> 1
+  | M64 -> 1
+
 
 type felem (s:field_spec) = lbuffer (limb s) (nlimb s)
 type felem_wide (s:field_spec) = lbuffer (wide s) (nlimb s)
 
 noextract 
 val as_nat: #s:field_spec -> h:mem -> e:felem s-> GTot nat 
-let as_nat #s h e = 
+let as_nat #s h (e:felem s) = 
   match s with
-  | M32 -> admit()
+  | M32 -> F32.as_nat h e
   | M64 -> F64.as_nat h e
   
 inline_for_extraction
@@ -55,8 +62,8 @@ val create_felem: s:field_spec -> StackInline (felem s)
 			    /\ as_nat h1 f == 0))
 let create_felem s = 
   match s with
-  | M32 -> admit()
-  | M64 -> F64.create_felem ()
+  | M32 -> (F32.create_felem ()) <: felem s
+  | M64 -> (F64.create_felem ()) <: felem s
 
 
 inline_for_extraction
@@ -65,7 +72,7 @@ val carry_felem: #s:field_spec -> f:felem s -> Stack unit
 		   (ensures (fun h0 _ h1 -> modifies (loc_buffer f) h0 h1))
 let carry_felem #s f =
   match s with
-  | M32 -> admit()
+  | M32 -> F32.carry_felem f
   | M64 -> F64.carry_felem f
 
 inline_for_extraction
@@ -74,7 +81,7 @@ val carry_top_felem: #s:field_spec -> f:felem s -> Stack unit
 		   (ensures (fun h0 _ h1 -> modifies (loc_buffer f) h0 h1))
 let carry_top_felem #s f =
   match s with
-  | M32 -> admit()
+  | M32 -> F32.carry_top_felem f
   | M64 -> F64.carry_top_felem f
 
 inline_for_extraction
@@ -83,7 +90,7 @@ val load_felem: #s:field_spec -> f:felem s -> lo:uint64 -> hi:uint64 -> Stack un
 		   (ensures (fun h0 _ h1 -> modifies (loc_buffer f) h0 h1))
 let load_felem (#s:field_spec) (f:felem s) (lo:uint64) (hi:uint64) = 
   match s with
-  | M32 -> admit()
+  | M32 -> F32.load_felem f lo hi
   | M64 -> F64.load_felem f lo hi
 
 inline_for_extraction
@@ -92,7 +99,7 @@ val store_felem: #s:field_spec -> f:felem s -> Stack (lo:uint64 * hi:uint64)
 		   (ensures (fun h0 _ h1 -> h0 == h1))
 let store_felem (#s:field_spec) (f:felem s) =
   match s with
-  | M32 -> admit()
+  | M32 -> F32.store_felem f
   | M64 -> F64.store_felem f 
 
 inline_for_extraction
@@ -101,7 +108,7 @@ val set_bit: #s:field_spec -> f:felem s -> i:size_t{size_v i < 130} -> Stack uni
 		   (ensures (fun h0 _ h1 -> modifies (loc_buffer f) h0 h1))
 let set_bit (#s:field_spec) (f:felem s) (i:size_t{size_v i < 130}) = 
   match s with
-  | M32 -> admit()
+  | M32 -> F32.set_bit f i
   | M64 -> F64.set_bit f i
 
 inline_for_extraction
@@ -110,7 +117,7 @@ val set_bit128: #s:field_spec -> f:felem s -> Stack unit
 		   (ensures (fun h0 _ h1 -> modifies (loc_buffer f) h0 h1))
 let set_bit128 (#s:field_spec) (f:felem s) = 
   match s with
-  | M32 -> admit()
+  | M32 -> F32.set_bit128 f
   | M64 -> F64.set_bit128 f
 
 
@@ -120,17 +127,17 @@ val set_zero: #s:field_spec -> f:felem s -> Stack unit
 		   (ensures (fun h0 _ h1 -> modifies (loc_buffer f) h0 h1))
 let set_zero (#s:field_spec) (f:felem s) = 
   match s with
-  | M32 -> admit()
+  | M32 -> F32.set_zero f
   | M64 -> F64.set_zero f
 
 inline_for_extraction
-val smul20_felem: #s:field_spec -> f1:felem s -> f2:felem s-> Stack unit
+val smul_top_felem: #s:field_spec -> f1:felem s -> f2:felem s-> Stack unit
                    (requires (fun h -> live h f1 /\ live h f2))
 		   (ensures (fun h0 _ h1 -> modifies (loc_buffer f1) h0 h1))
-let smul20_felem #s f1 f2 = 
+let smul_top_felem #s f1 f2 = 
   match s with
-  | M32 -> admit()
-  | M64 -> F64.smul20_felem f1 f2
+  | M32 -> F32.smul_top_felem f1 f2
+  | M64 -> F64.smul_top_felem f1 f2
 
 
 inline_for_extraction
@@ -139,7 +146,7 @@ val fadd_mul_felem: #s:field_spec -> acc:felem s -> f1:felem s -> f2:felem s -> 
 		   (ensures (fun h0 _ h1 -> modifies (loc_buffer acc) h0 h1))
 let fadd_mul_felem #s acc f1 f2 f2_20 =
   match s with
-  | M32 -> admit()
+  | M32 -> F32.fadd_mul_felem acc f1 f2 f2_20
   | M64 -> F64.fadd_mul_felem acc f1 f2 f2_20
 
 inline_for_extraction
@@ -148,6 +155,6 @@ val add_felem: #s:field_spec -> f1:felem s -> f2:felem s -> Stack unit
 		   (ensures (fun h0 _ h1 -> modifies (loc_buffer f1) h0 h1))
 let add_felem #s f1 f2=
   match s with
-  | M32 -> admit()
-  | M64 -> admit(); F64.add_felem f1 f2 
+  | M32 -> F32.add_felem f1 f2 
+  | M64 -> F64.add_felem f1 f2 
 
